src/cnf/clause.lean
@@ -16,10 +16,10 @@ import data.list.basic
 universe u
 
 -- Represents the parametric type of the variable stored in the literal
-variables {V : Type u} [decidable_eq V] [inhabited V]
+variables {V : Type*} [decidable_eq V] [inhabited V]
 
 /- Disjunctive clauses are lists of literals, joined by logical ORs. -/
-def clause (V : Type u) := list (literal V)
+def clause (V : Type*) := list (literal V)
 
 -- Note that the above definition allows for duplication of literals, whereas
 -- a set definition would not. Lists also allow for computable functions,
@@ -67,37 +67,37 @@ by apply_instance
 
 -- Note: protected b/c many constructs will have an evaluation def
 /- To evaluate the clause, fold false along until a true evaluation is found -/
-protected def eval (α : assignment V) (c : clause V) : bool :=
-  c.foldr (λ l b, b || (l.eval α)) ff
+protected def eval (τ : assignment V) (c : clause V) : bool :=
+  c.foldr (λ l b, b || (l.eval τ)) ff
 
 -- Proving properties of the fold operation
-lemma eval_op_left_comm (α : assignment V) : 
-  left_commutative (λ (l : literal V) (b : bool), b || (l.eval α)) :=
+lemma eval_op_left_comm (τ : assignment V) : 
+  left_commutative (λ (l : literal V) (b : bool), b || (l.eval τ)) :=
 assume l₁ l₂ b, by simp [bool.bor_comm, bool.bor_assoc]
 
-@[simp] theorem eval_nil (α : assignment V) : clause.eval α [] = ff := rfl
+@[simp] theorem eval_nil (τ : assignment V) : clause.eval τ [] = ff := rfl
 
-@[simp] theorem eval_singleton (α : assignment V) (l : literal V) : 
-  clause.eval α [l] = l.eval α :=
+@[simp] theorem eval_singleton (τ : assignment V) (l : literal V) : 
+  clause.eval τ [l] = l.eval τ :=
 by simp only [clause.eval, foldr, ff_bor]
 
 -- TODO make this, and other similarly-named theorems, protected?
-theorem eval_cons (α : assignment V) (l : literal V) (c : clause V) : 
-  clause.eval α (l :: c) = (literal.eval α l) || (clause.eval α c) :=
+theorem eval_cons (τ : assignment V) (l : literal V) (c : clause V) : 
+  clause.eval τ (l :: c) = (literal.eval τ l) || (clause.eval τ c) :=
 by simp only [clause.eval, foldr, bool.bor_comm]
 
-theorem eval_append (α : assignment V) (c₁ c₂ : clause V) :
-  clause.eval α (c₁ ++ c₂) = c₁.eval α || c₂.eval α :=
+theorem eval_append (τ : assignment V) (c₁ c₂ : clause V) :
+  clause.eval τ (c₁ ++ c₂) = c₁.eval τ || c₂.eval τ :=
 begin
   unfold clause.eval,
   rw foldr_append,
-  cases foldr (λ l b, b || literal.eval α l) ff c₂,
+  cases foldr (λ l b, b || literal.eval τ l) ff c₂,
   { rw bor_ff },
   { rw [bor_tt, foldr_bor_tt] }
 end
 
-theorem eval_tt_iff_exists_literal_eval_tt {α : assignment V} {c : clause V} : 
-  clause.eval α c = tt ↔ ∃ l ∈ c, literal.eval α l = tt :=
+theorem eval_tt_iff_exists_literal_eval_tt {τ : assignment V} {c : clause V} : 
+  c.eval τ = tt ↔ ∃ l ∈ c, literal.eval τ l = tt :=
 begin
   split,
   { induction c with l ls ih,
@@ -115,16 +115,16 @@ begin
       { simp [eval_cons, ih hds] } } }
 end
 
-theorem ne_nil_of_eval_tt {α : assignment V} {c : clause V} :
-  c.eval α = tt → c ≠ [] :=
+theorem ne_nil_of_eval_tt {τ : assignment V} {c : clause V} :
+  c.eval τ = tt → c ≠ [] :=
 begin
   intro h,
   rcases eval_tt_iff_exists_literal_eval_tt.mp h with ⟨l, hmem, _⟩,
   exact ne_nil_of_mem hmem
 end
 
-theorem eval_ff_iff_forall_literal_eval_ff {α : assignment V} {c : clause V} : 
-  clause.eval α c = ff ↔ ∀ l ∈ c, literal.eval α l = ff :=
+theorem eval_ff_iff_forall_literal_eval_ff {τ : assignment V} {c : clause V} : 
+  clause.eval τ c = ff ↔ ∀ l ∈ c, literal.eval τ l = ff :=
 begin
   split,
   { induction c with l ls ih,
@@ -136,25 +136,25 @@ begin
     { rw eval_nil, tautology },
     { intro h,
       simp [eval_cons, h l (mem_cons_self l ls)],
-      have : ∀ (m : literal V), m ∈ ls → literal.eval α m = ff,
+      have : ∀ (m : literal V), m ∈ ls → literal.eval τ m = ff,
       { intros m hm, exact h m (mem_cons_of_mem l hm) },
       exact ih this } }
 end
 
 theorem eval_tautology {c : clause V} {l : literal V} : 
-  l ∈ c → l.flip ∈ c → ∀ (α : assignment V), clause.eval α c = tt :=
+  l ∈ c → l.flip ∈ c → ∀ (τ : assignment V), clause.eval τ c = tt :=
 begin
-  intros hl hlf α,
+  intros hl hlf τ,
   apply eval_tt_iff_exists_literal_eval_tt.mpr,
-  cases h : (literal.eval α l),
+  cases h : (literal.eval τ l),
   { use [l.flip, hlf, eval_flip_of_eval h] },
   { use [l, hl, h] }
 end
 
 -- Evaluation of subsets and sublists tie in to evaluation nicely
 
-theorem eval_tt_of_subset_eval_tt {α : assignment V} {c₁ c₂ : clause V} :
-  c₁ ⊆ c₂ → clause.eval α c₁ = tt → clause.eval α c₂ = tt :=
+theorem eval_tt_of_subset_eval_tt {τ : assignment V} {c₁ c₂ : clause V} :
+  c₁ ⊆ c₂ → clause.eval τ c₁ = tt → clause.eval τ c₂ = tt :=
 begin
   intros h₁ h₂,
   apply eval_tt_iff_exists_literal_eval_tt.mpr,
@@ -162,8 +162,8 @@ begin
   use [l, h₁ hl, he]
 end
 
-theorem eval_ff_of_superset_eval_ff {α : assignment V} {c₁ c₂ : clause V} :
-  c₁ ⊆ c₂ → clause.eval α c₂ = ff → clause.eval α c₁ = ff :=
+theorem eval_ff_of_superset_eval_ff {τ : assignment V} {c₁ c₂ : clause V} :
+  c₁ ⊆ c₂ → clause.eval τ c₂ = ff → clause.eval τ c₁ = ff :=
 begin
   intros h₁ h₂,
   apply eval_ff_iff_forall_literal_eval_ff.mpr,
@@ -172,33 +172,33 @@ begin
   exact h₂ l (h₁ hl)
 end
 
-theorem eval_tt_of_sublist_eval_tt {α : assignment V} {c₁ c₂ : clause V} :
-  c₁ <+ c₂ → clause.eval α c₁ = tt → clause.eval α c₂ = tt :=
+theorem eval_tt_of_sublist_eval_tt {τ : assignment V} {c₁ c₂ : clause V} :
+  c₁ <+ c₂ → clause.eval τ c₁ = tt → clause.eval τ c₂ = tt :=
 assume h₁, eval_tt_of_subset_eval_tt (sublist.subset h₁)
 
-theorem eval_ff_of_superlist_eval_ff {α : assignment V} {c₁ c₂ : clause V} :
-  c₁ <+ c₂ → clause.eval α c₂ = ff → clause.eval α c₁ = ff :=
+theorem eval_ff_of_superlist_eval_ff {τ : assignment V} {c₁ c₂ : clause V} :
+  c₁ <+ c₂ → clause.eval τ c₂ = ff → clause.eval τ c₁ = ff :=
 assume h₁, eval_ff_of_superset_eval_ff (sublist.subset h₁)
 
 theorem eval_tt_cons_of_eval_tt 
-  {α : assignment V} {c : clause V} (l : literal V) :
-  clause.eval α c = tt → clause.eval α (l :: c) = tt :=
+  {τ : assignment V} {c : clause V} (l : literal V) :
+  clause.eval τ c = tt → clause.eval τ (l :: c) = tt :=
 assume h, eval_tt_of_sublist_eval_tt (sublist_cons l c) h
 
 theorem eval_ff_of_eval_ff_cons 
-  {α : assignment V} {c : clause V} {l : literal V} :
-  clause.eval α (l :: c) = ff → clause.eval α c = ff :=
+  {τ : assignment V} {c : clause V} {l : literal V} :
+  clause.eval τ (l :: c) = ff → clause.eval τ c = ff :=
 assume h, eval_ff_of_superlist_eval_ff (sublist_cons l c) h
 
 /-! ### Counting -/
 
-/- Counts the number of literals that evaluate to true, under α -/
-protected def count_tt (α : assignment V) (c : clause V) : nat :=
-  c.countp (literal.is_true α)
+/- Counts the number of literals that evaluate to true, under τ -/
+protected def count_tt (τ : assignment V) (c : clause V) : nat :=
+  c.countp (literal.is_true τ)
 
-/- Counts the number of literals that evaluate to false, under α -/
-protected def count_ff (α : assignment V) (c : clause V) : nat :=
-  c.countp (literal.is_false α)
+/- Counts the number of literals that evaluate to false, under τ -/
+protected def count_ff (τ : assignment V) (c : clause V) : nat :=
+  c.countp (literal.is_false τ)
 
 /- Counts the number of positive literals in the clause -/
 def count_pos (c : clause V) : nat :=
@@ -208,18 +208,18 @@ def count_pos (c : clause V) : nat :=
 def count_neg (c : clause V) : nat :=
   c.countp literal.is_neg
 
-@[simp] lemma count_tt_nil (α : assignment V) : clause.count_tt α [] = 0 := rfl
-@[simp] lemma count_ff_nil (α : assignment V) : clause.count_ff α [] = 0 := rfl
+@[simp] lemma count_tt_nil (τ : assignment V) : clause.count_tt τ [] = 0 := rfl
+@[simp] lemma count_ff_nil (τ : assignment V) : clause.count_ff τ [] = 0 := rfl
 @[simp] lemma count_pos_nil : count_pos ([] : clause V) = 0 := rfl
 @[simp] lemma count_neg_nil : count_neg ([] : clause V) = 0 := rfl
 
-@[simp] theorem count_tt_singleton (α : assignment V) (l : literal V) :
-  clause.count_tt α [l] = cond (l.eval α) 1 0 :=
-by cases h : (l.eval α); { simp [h, clause.count_tt, literal.is_true] }
+@[simp] theorem count_tt_singleton (τ : assignment V) (l : literal V) :
+  clause.count_tt τ [l] = cond (l.eval τ) 1 0 :=
+by cases h : (l.eval τ); { simp [h, clause.count_tt, literal.is_true] }
 
-@[simp] theorem count_ff_singleton (α : assignment V) (l : literal V) :
-  clause.count_ff α [l] = cond (l.eval α) 0 1 :=
-by cases h : (l.eval α); { simp [h, clause.count_ff, literal.is_false] }
+@[simp] theorem count_ff_singleton (τ : assignment V) (l : literal V) :
+  clause.count_ff τ [l] = cond (l.eval τ) 0 1 :=
+by cases h : (l.eval τ); { simp [h, clause.count_ff, literal.is_false] }
 
 @[simp] theorem count_pos_singleton (l : literal V) :
   count_pos [l] = cond l.is_pos 1 0 :=
@@ -229,14 +229,14 @@ by cases l; simp [count_pos, literal.is_pos]
   count_neg [l] = cond l.is_neg 1 0 :=
 by cases l; simp [count_neg, literal.is_neg]
 
-theorem count_tt_cons (α : assignment V) (l : literal V) (c : clause V) :
-  clause.count_tt α (l :: c) = cond (l.eval α) (1 + c.count_tt α) (c.count_tt α) :=
-by cases h : (literal.eval α l); 
+theorem count_tt_cons (τ : assignment V) (l : literal V) (c : clause V) :
+  clause.count_tt τ (l :: c) = cond (l.eval τ) (1 + c.count_tt τ) (c.count_tt τ) :=
+by cases h : (literal.eval τ l); 
   { simp [h, literal.is_true, clause.count_tt, add_comm] }
 
-theorem count_ff_cons (α : assignment V) (l : literal V) (c : clause V) :
-  clause.count_ff α (l :: c) = cond (l.eval α) (c.count_ff α) (1 + c.count_ff α) :=
-by cases h : (literal.eval α l);
+theorem count_ff_cons (τ : assignment V) (l : literal V) (c : clause V) :
+  clause.count_ff τ (l :: c) = cond (l.eval τ) (c.count_ff τ) (1 + c.count_ff τ) :=
+by cases h : (literal.eval τ l);
   { simp [h, literal.is_false, clause.count_ff, add_comm] }
 
 theorem count_pos_cons (l : literal V) (c : clause V) :
@@ -247,24 +247,24 @@ theorem count_neg_cons (l : literal V) (c : clause V) :
   count_neg (l :: c) = cond l.is_neg (1 + c.count_neg) c.count_neg :=
 by cases l; { simp [count_neg, literal.is_neg, add_comm] }
 
-theorem count_tt_append (α : assignment V) (c₁ c₂ : clause V) :
-  clause.count_tt α (c₁ ++ c₂) = clause.count_tt α c₁ + clause.count_tt α c₂ :=
+theorem count_tt_append (τ : assignment V) (c₁ c₂ : clause V) :
+  clause.count_tt τ (c₁ ++ c₂) = clause.count_tt τ c₁ + clause.count_tt τ c₂ :=
 begin
   induction c₁ with l ls ih,
   { simp only [count_tt_nil, zero_add, nil_append] },
-  { cases h : (literal.eval α l);
+  { cases h : (literal.eval τ l);
     { simp [count_tt_cons, h, ih, add_assoc] } }
 end
 
 -- Can make analogous append theorems for each of the others
 
 -- All the above four functions are capped by the length of the clause
-theorem count_tt_le_length (α : assignment V) (c : clause V) :
-  c.count_tt α ≤ c.length :=
+theorem count_tt_le_length (τ : assignment V) (c : clause V) :
+  c.count_tt τ ≤ c.length :=
 by simp only [clause.count_tt, countp_eq_length_filter, length_filter]
 
-theorem count_ff_le_length (α : assignment V) (c : clause V) : 
-  c.count_ff α ≤ c.length :=
+theorem count_ff_le_length (τ : assignment V) (c : clause V) : 
+  c.count_ff τ ≤ c.length :=
 by simp only [clause.count_ff, countp_eq_length_filter, length_filter]
 
 theorem count_pos_le_length (c : clause V) : c.count_pos ≤ c.length :=
@@ -274,27 +274,27 @@ theorem count_neg_le_length (c : clause V) : c.count_neg ≤ c.length :=
 by simp only [count_neg, countp_eq_length_filter, length_filter]
 
 -- count_tt and count_ff are complements of each other
-theorem count_tt_plus_count_ff_eq_length (α : assignment V) (c : clause V) :
-  c.count_tt α + c.count_ff α = c.length :=
+theorem count_tt_plus_count_ff_eq_length (τ : assignment V) (c : clause V) :
+  c.count_tt τ + c.count_ff τ = c.length :=
 begin
   induction c with l ls ih,
   { simp },
-  { cases h : (l.eval α);
+  { cases h : (l.eval τ);
     simp [count_tt_cons, count_ff_cons, h, ← ih],
     { rw add_assoc,
-      rw add_comm (clause.count_ff α ls) 1 },
-    { rw add_comm (clause.count_tt α ls + clause.count_ff α ls) 1,
+      rw add_comm (clause.count_ff τ ls) 1 },
+    { rw add_comm (clause.count_tt τ ls + clause.count_ff τ ls) 1,
       rw ← add_assoc } }
 end
 
-theorem count_tt_eq_length_sub_count_ff (α : assignment V) (c : clause V) :
-  c.count_tt α = c.length - c.count_ff α :=
-eq_tsub_of_add_eq (count_tt_plus_count_ff_eq_length α c)
+theorem count_tt_eq_length_sub_count_ff (τ : assignment V) (c : clause V) :
+  c.count_tt τ = c.length - c.count_ff τ :=
+eq_tsub_of_add_eq (count_tt_plus_count_ff_eq_length τ c)
 
-theorem count_ff_eq_length_sub_count_tt (α : assignment V) (c : clause V) :
-  c.count_ff α = c.length - c.count_tt α :=
+theorem count_ff_eq_length_sub_count_tt (τ : assignment V) (c : clause V) :
+  c.count_ff τ = c.length - c.count_tt τ :=
 begin
-  have := count_tt_plus_count_ff_eq_length α c,
+  have := count_tt_plus_count_ff_eq_length τ c,
   rw add_comm at this,
   exact eq_tsub_of_add_eq this
 end
@@ -326,8 +326,8 @@ begin
 end
 
 -- Note: A good countp lemma may reduce the forward direction
-theorem count_tt_eq_zero_iff_eval_ff {α : assignment V} {c : clause V} :
-  c.eval α = ff ↔ c.count_tt α = 0 :=
+theorem count_tt_eq_zero_iff_eval_ff {τ : assignment V} {c : clause V} :
+  c.eval τ = ff ↔ c.count_tt τ = 0 :=
 begin
   split,
   { induction c with l ls ih,
@@ -338,7 +338,7 @@ begin
   { induction c with l ls ih,
     { simp },
     { simp [eval_cons, count_tt_cons],
-      have : 1 + clause.count_tt α ls ≠ 0,
+      have : 1 + clause.count_tt τ ls ≠ 0,
       { rw add_comm,
         rw ← nat.succ_eq_add_one,
         exact nat.succ_ne_zero _ },
@@ -348,8 +348,8 @@ begin
       exact and.intro this (ih h) } }
 end
 
-theorem count_tt_eval_tt_iff_gt_zero {α : assignment V} {c : clause V} :
-  c.eval α = tt ↔ clause.count_tt α c > 0 :=
+theorem count_tt_eval_tt_iff_gt_zero {τ : assignment V} {c : clause V} :
+  c.eval τ = tt ↔ clause.count_tt τ c > 0 :=
 begin
   split,
   { intro h,
@@ -364,105 +364,105 @@ end
 
 -- For any assignment and variables, there is a false clause on those variables
 -- Simply map each variable in the list to the literal which evaluates to false
-def falsify (α : assignment V) (l : list V) : clause V :=
-l.map (λ v, cond (α v) (Neg v) (Pos v))
+def falsify (τ : assignment V) (l : list V) : clause V :=
+l.map (λ v, cond (τ v) (Neg v) (Pos v))
 
 -- For any assignment and variables, there is a true clause on those variables
 -- Note: there is no such clause for the empty set of variables
-def truthify (α : assignment V) (l : list V) : clause V :=
-l.map (λ v, cond (α v) (Pos v) (Neg v))
+def truthify (τ : assignment V) (l : list V) : clause V :=
+l.map (λ v, cond (τ v) (Pos v) (Neg v))
 
-@[simp] lemma falsify_nil (α : assignment V) : falsify α [] = [] := rfl
-@[simp] lemma truthify_nil (α : assignment V) : truthify α [] = [] := rfl
+@[simp] lemma falsify_nil (τ : assignment V) : falsify τ [] = [] := rfl
+@[simp] lemma truthify_nil (τ : assignment V) : truthify τ [] = [] := rfl
 
-@[simp] lemma falsify_singleton (α : assignment V) (v : V) :
-  falsify α [v] = cond (α v) [Neg v] [Pos v] :=
-by cases h : α v; { simp [h, falsify] }
+@[simp] lemma falsify_singleton (τ : assignment V) (v : V) :
+  falsify τ [v] = cond (τ v) [Neg v] [Pos v] :=
+by cases h : τ v; { simp [h, falsify] }
 
-@[simp] lemma truthify_singleton (α : assignment V) (v : V) :
-  truthify α [v] = cond (α v) [Pos v] [Neg v] :=
-by cases h : α v; { simp [h, truthify] }
+@[simp] lemma truthify_singleton (τ : assignment V) (v : V) :
+  truthify τ [v] = cond (τ v) [Pos v] [Neg v] :=
+by cases h : τ v; { simp [h, truthify] }
 
-theorem falsify_cons (α : assignment V) (v : V) (vs : list V) :
-  falsify α (v :: vs) = cond (α v) (Neg v :: falsify α vs)
-                                   (Pos v :: falsify α vs) :=
-by cases h : α v; { simp [falsify, map_cons, h] }
+theorem falsify_cons (τ : assignment V) (v : V) (vs : list V) :
+  falsify τ (v :: vs) = cond (τ v) (Neg v :: falsify τ vs)
+                                   (Pos v :: falsify τ vs) :=
+by cases h : τ v; { simp [falsify, map_cons, h] }
 
-theorem truthify_cons (α : assignment V) (v : V) (vs : list V) :
-  truthify α (v :: vs) = cond (α v) (Pos v :: truthify α vs)
-                                    (Neg v :: truthify α vs) :=
-by cases h : α v; { simp [truthify, map_cons, h] }
+theorem truthify_cons (τ : assignment V) (v : V) (vs : list V) :
+  truthify τ (v :: vs) = cond (τ v) (Pos v :: truthify τ vs)
+                                    (Neg v :: truthify τ vs) :=
+by cases h : τ v; { simp [truthify, map_cons, h] }
 
-theorem falsify_eval_ff (α : assignment V) (l : list V) :
-  clause.eval α (falsify α l) = ff :=
+theorem falsify_eval_ff (τ : assignment V) (l : list V) :
+  clause.eval τ (falsify τ l) = ff :=
 begin
   induction l with v vs ih,
   { rw falsify_nil, rw eval_nil },
-  { cases h : (α v);
+  { cases h : (τ v);
     { simp [falsify_cons, h, eval_cons, literal.eval, ih] } }
 end
 
-theorem truthify_eval_tt (α : assignment V) {l : list V} (hl : l ≠ []) : 
-  clause.eval α (truthify α l) = tt :=
+theorem truthify_eval_tt (τ : assignment V) {l : list V} (hl : l ≠ []) : 
+  clause.eval τ (truthify τ l) = tt :=
 begin
   induction l with v vs ih,
   { contradiction },
-  { cases h : (α v);
+  { cases h : (τ v);
     { simp [truthify_cons, h, literal.eval, eval_cons] } }
 end
 
-theorem flip_truthify_eq_falsify (α : assignment V) (l : list V) : 
-  map literal.flip (truthify α l) = falsify α l :=
+theorem flip_truthify_eq_falsify (τ : assignment V) (l : list V) : 
+  map literal.flip (truthify τ l) = falsify τ l :=
 begin
   induction l with v vs ih,
   { simp },
-  { cases h : (α v);
+  { cases h : (τ v);
     { simp [h, literal.eval, ih, literal.flip, truthify_cons, falsify_cons] } }
 end
 
 -- If falsify/truthify become type (fin)set, these theorems aren't needed
-theorem falsify_map_var_eq (α : assignment V) (l : list V) : 
-  map var (falsify α l) = l :=
+theorem falsify_map_var_eq (τ : assignment V) (l : list V) : 
+  map var (falsify τ l) = l :=
 begin
   induction l with v vs ih,
   { simp only [falsify_nil, map_nil] },
-  { cases h : (α v);
+  { cases h : (τ v);
     { simp only [falsify_cons, map_cons, h, var, 
         true_and, eq_self_iff_true, cond],
       exact ih } }
 end
 
-theorem truthify_map_var_eq (α : assignment V) (l : list V) :
-  map var (truthify α l) = l :=
+theorem truthify_map_var_eq (τ : assignment V) (l : list V) :
+  map var (truthify τ l) = l :=
 begin
   induction l with v vs ih,
   { simp only [truthify_nil, map_nil] },
-  { cases h : (α v);
+  { cases h : (τ v);
     { simp only [truthify_cons, map_cons, h, var, 
         true_and, eq_self_iff_true, cond],
       exact ih } }
 end
 
-theorem count_tt_falsify (α : assignment V) (l : list V) :
-  clause.count_tt α (falsify α l) = 0 :=
-count_tt_eq_zero_iff_eval_ff.mp (falsify_eval_ff α l)
+theorem count_tt_falsify (τ : assignment V) (l : list V) :
+  clause.count_tt τ (falsify τ l) = 0 :=
+count_tt_eq_zero_iff_eval_ff.mp (falsify_eval_ff τ l)
 
-lemma count_tt_truthify (α : assignment V) (l : list V) :
-  clause.count_tt α (truthify α l) = length l :=
+lemma count_tt_truthify (τ : assignment V) (l : list V) :
+  clause.count_tt τ (truthify τ l) = length l :=
 begin
   induction l with v vs ih,
   { simp },
-  { cases h : α v;
+  { cases h : τ v;
     { simp [truthify_cons, count_tt_cons, literal.eval, h, ih, add_comm] } }
 end
 
 -- Falsify negates those literals that, if positive, are true
-theorem count_tt_pos_eq_count_neg_falsify (α : assignment V) (l : list V) :
-  clause.count_tt α (map Pos l) = count_neg (falsify α l) :=
+theorem count_tt_pos_eq_count_neg_falsify (τ : assignment V) (l : list V) :
+  clause.count_tt τ (map Pos l) = count_neg (falsify τ l) :=
 begin
   induction l with v vs ih,
   { simp },
-  { cases h : (α v);
+  { cases h : (τ v);
     { simp [map_cons, count_tt_cons, falsify_cons, count_neg_cons, 
         literal.eval, h, ih, literal.is_neg] } }
 end
@@ -476,13 +476,13 @@ theorem count_neg_sublist {c₁ c₂ : clause V} :
   c₁ <+ c₂ → c₁.count_neg ≤ c₂.count_neg :=
 assume h, by simp [count_neg, sublist.countp_le literal.is_neg h]
 
-theorem count_tt_sublist (α : assignment V) {c₁ c₂ : clause V} :
-  c₁ <+ c₂ → c₁.count_tt α ≤ c₂.count_tt α :=
-assume h, by simp [clause.count_tt, sublist.countp_le (literal.is_true α) h]
+theorem count_tt_sublist (τ : assignment V) {c₁ c₂ : clause V} :
+  c₁ <+ c₂ → c₁.count_tt τ ≤ c₂.count_tt τ :=
+assume h, by simp [clause.count_tt, sublist.countp_le (literal.is_true τ) h]
 
-theorem count_ff_sublist (α : assignment V) {c₁ c₂ : clause V} :
-  c₁ <+ c₂ → c₁.count_ff α ≤ c₂.count_ff α :=
-assume h, by simp [clause.count_ff, sublist.countp_le (literal.is_false α) h]
+theorem count_ff_sublist (τ : assignment V) {c₁ c₂ : clause V} :
+  c₁ <+ c₂ → c₁.count_ff τ ≤ c₂.count_ff τ :=
+assume h, by simp [clause.count_ff, sublist.countp_le (literal.is_false τ) h]
 
 theorem pos_count_pos_iff_exists_pos {c : clause V} :
   c.count_pos > 0 ↔ ∃ l ∈ c, literal.is_pos l :=
@@ -492,12 +492,12 @@ theorem pos_count_neg_iff_exists_neg {c : clause V} :
   c.count_neg > 0 ↔ ∃ l ∈ c, literal.is_neg l :=
 by simp [count_neg, countp_pos]
 
-theorem pos_count_tt_iff_exists_tt {α : assignment V} {c : clause V} :
-  c.count_tt α > 0 ↔ ∃ l ∈ c, literal.is_true α l :=
+theorem pos_count_tt_iff_exists_tt {τ : assignment V} {c : clause V} :
+  c.count_tt τ > 0 ↔ ∃ l ∈ c, literal.is_true τ l :=
 by simp [clause.count_tt, countp_pos]
 
-theorem pos_count_ff_iff_exists_ff {α : assignment V} {c : clause V} :
-  c.count_ff α > 0 ↔ ∃ l ∈ c, literal.is_false α l :=
+theorem pos_count_ff_iff_exists_ff {τ : assignment V} {c : clause V} :
+  c.count_ff τ > 0 ↔ ∃ l ∈ c, literal.is_false τ l :=
 by simp [clause.count_ff, countp_pos]
 
 /-! # Flip counting -/
@@ -560,13 +560,13 @@ begin
     { simp [flip_flip, nat.zero_lt_one_add] } }
 end
 
-theorem count_flips_falsify_eq_count_tt (α : assignment V) (c : clause V) :
-  count_flips c (falsify α (map var c)) = clause.count_tt α c :=
+theorem count_flips_falsify_eq_count_tt (τ : assignment V) (c : clause V) :
+  count_flips c (falsify τ (map var c)) = clause.count_tt τ c :=
 begin
   induction c with l ls ih,
   { simp },
   { cases l;
-    { cases h : (α l);
+    { cases h : (τ l);
       { simp [map_cons, falsify_cons, count_tt_cons, count_flips_cons, 
           literal.eval, h, var, literal.flip, ih] } } }
 end
@@ -574,21 +574,21 @@ end
 /-! ## Parity reasoning for evaluation -/
 
 theorem eval_tt_of_tt_ne_neg_of_map_var_eq 
-  {α : assignment V} {l : list V} {c : clause V} :
-  map var c = l → clause.count_tt α (map Pos l) ≠ count_neg c → c.eval α = tt :=
+  {τ : assignment V} {l : list V} {c : clause V} :
+  map var c = l → clause.count_tt τ (map Pos l) ≠ count_neg c → c.eval τ = tt :=
 begin
   induction l with v vs ih generalizing c,
   { rw map_eq_nil, rintro rfl, contradiction },
   { intros hc hne,
     rcases exists_cons_of_map_cons hc with ⟨l, ls, rfl, hl, hls⟩,
     cases l,
-    { cases h : α v,
+    { cases h : τ v,
       { simp [map_cons, count_tt_cons, count_neg_cons, 
           literal.is_neg, literal.eval, h] at hne,
         exact eval_tt_cons_of_eval_tt _ (ih hls hne) },
       { unfold var at hl,
         simp [eval_cons, literal.eval, h, hl] } },
-    { cases h : α v,
+    { cases h : τ v,
       { unfold var at hl,
         simp [eval_cons, literal.eval, h, hl] },
       { simp [map_cons, count_tt_cons, count_neg_cons, 
@@ -599,21 +599,21 @@ end
 -- Basically the same proof here as the one above
 -- Take complement of count_ff, etc. to get above premises?
 theorem eval_tt_of_ff_ne_pos_of_map_var_eq 
-  {α : assignment V} {l : list V} {c : clause V} : map var c = l 
-    → clause.count_ff α (map Pos l) ≠ count_pos c → c.eval α = tt :=
+  {τ : assignment V} {l : list V} {c : clause V} : map var c = l 
+    → clause.count_ff τ (map Pos l) ≠ count_pos c → c.eval τ = tt :=
 begin
   induction l with v vs ih generalizing c,
   { rw map_eq_nil, rintro rfl, contradiction },
   { intros hc hne,
     rcases exists_cons_of_map_cons hc with ⟨l, ls, rfl, hl, hls⟩,
     cases l,
-    { cases h : α v,
+    { cases h : τ v,
       { simp [map_cons, count_ff_cons, count_pos_cons, 
           literal.is_pos, literal.eval, h] at hne,
         exact eval_tt_cons_of_eval_tt _ (ih hls hne) },
       { unfold var at hl,
         simp [eval_cons, literal.eval, h, hl] } },
-    { cases h : α v,
+    { cases h : τ v,
       { unfold var at hl,
         simp [eval_cons, literal.eval, h, hl] },
       { simp [map_cons, count_ff_cons, count_pos_cons, 
@@ -623,32 +623,32 @@ end
 
 -- Corollary of the above wrt parity reasoning
 theorem eval_tt_of_opposite_parity 
-  {α : assignment V} {l : list V} {c : clause V} : map var c = l 
-    → nat.bodd (clause.count_tt α (map Pos l)) ≠ nat.bodd (count_neg c) 
-    → clause.eval α c = tt :=
+  {τ : assignment V} {l : list V} {c : clause V} : map var c = l 
+    → nat.bodd (clause.count_tt τ (map Pos l)) ≠ nat.bodd (count_neg c) 
+    → clause.eval τ c = tt :=
 assume hc hcount, 
   eval_tt_of_tt_ne_neg_of_map_var_eq hc (ne_of_apply_ne nat.bodd hcount)
 
 -- Parity reasoning based on flips rather than negs
 -- If a clause evaluates to false, then any clause that can be made by flipping a
 -- variable in that clause will evaluate to true
-theorem eval_tt_of_ne_flips {α : assignment V} {c₁ c₂ : clause V} :
+theorem eval_tt_of_ne_flips {τ : assignment V} {c₁ c₂ : clause V} :
   map var c₁ = map var c₂ → 
-    clause.count_tt α c₁ ≠ count_flips c₁ c₂ → c₂.eval α = tt :=
+    clause.count_tt τ c₁ ≠ count_flips c₁ c₂ → c₂.eval τ = tt :=
 begin
   induction c₁ with l ls ih generalizing c₂,
   { simp },
   { intros hc₂ hne,
     rcases exists_map_cons_of_map_cons hc₂.symm with ⟨m, ms, rfl, hm, hms⟩,
     cases m,
-    { cases h : (α m),
+    { cases h : (τ m),
       { cases l;
         { unfold var at hm,
           simp [count_tt_cons, count_flips_cons, 
             literal.eval, literal.flip, ← hm, h] at hne,
           exact eval_tt_cons_of_eval_tt _ (ih hms.symm hne) } },
       { simp only [eval_cons, literal.eval, hm, h, tt_bor] } },
-    { cases h : (α m),
+    { cases h : (τ m),
       { simp only [eval_cons, literal.eval, hm, h, bnot, tt_bor] },
       { cases l;
         { unfold var at hm,
@@ -670,9 +670,23 @@ protected def vars : clause V → finset V
 @[simp] theorem vars_singleton (l : literal V) : clause.vars [l] = {l.var} :=
 by { unfold clause.vars, rw finset.union_empty }
 
+theorem mem_vars_cons_self (l : literal V) (c : clause V) :
+  l.var ∈ clause.vars (l :: c) :=
+begin
+  rw clause.vars,
+  exact finset.mem_union_left _ (finset.mem_singleton_self l.var)
+end
+
 theorem mem_vars_cons_of_mem_vars {c : clause V} (l : literal V) {v : V} : 
   v ∈ c.vars → v ∈ clause.vars (l :: c) :=
 assume h, finset.mem_union.mpr (or.inr h)
+
+theorem vars_append (c₁ c₂ : clause V) : (c₁ ++ c₂).vars = c₁.vars ∪ c₂.vars :=
+begin
+  induction c₁ with l ls ih,
+  { simp only [finset.empty_union, vars_nil, nil_append] },
+  { simp only [cons_append, clause.vars, ih, finset.union_assoc] }
+end 
 
 theorem mem_vars_of_mem {c : clause V} {l : literal V} : 
   l ∈ c → l.var ∈ c.vars :=
@@ -803,13 +817,14 @@ end clause
 
 namespace assignment
 
+open literal
 open clause
 
-theorem eval_eq_clause_of_eqod {α₁ α₂ : assignment V} {c : clause V} :
-  (α₁ ≡c.vars≡ α₂) → c.eval α₁ = c.eval α₂ :=
+theorem eval_eq_clause_of_eqod {τ₁ τ₂ : assignment V} {c : clause V} :
+  (τ₁ ≡c.vars≡ τ₂) → c.eval τ₁ = c.eval τ₂ :=
 begin
   intro h,
-  cases hev : (c.eval α₂),
+  cases hev : (c.eval τ₂),
   { rw eval_ff_iff_forall_literal_eval_ff at hev,
     apply eval_ff_iff_forall_literal_eval_ff.mpr,
     intros l hl,
@@ -820,9 +835,9 @@ begin
     exact htt ▸ eval_eq_of_eqod_of_var_mem h (mem_vars_of_mem hl) }
 end
 
--- Can replace α in count_tt if eqod
-theorem count_tt_eq_of_eqod {α₁ α₂ : assignment V} {c : clause V} :
-  (α₁ ≡c.vars≡ α₂) → clause.count_tt α₁ c = clause.count_tt α₂ c :=
+-- Can replace τ in count_tt if eqod
+theorem count_tt_eq_of_eqod {τ₁ τ₂ : assignment V} {c : clause V} :
+  (τ₁ ≡c.vars≡ τ₂) → clause.count_tt τ₁ c = clause.count_tt τ₂ c :=
 begin
   induction c with l ls ih,
   { simp only [count_tt_nil, eqod_nil, vars_nil, forall_true_left] },
@@ -836,5 +851,8 @@ begin
         this l (finset.mem_singleton_self l), ihred] } }
 end
 
+theorem count_tt_ite {τ₁ τ₂ : assignment V} (c : clause V) :
+  clause.count_tt (assignment.ite c.vars τ₁ τ₂) c = clause.count_tt τ₁ c :=
+count_tt_eq_of_eqod (ite_eqod τ₁ τ₂ c.vars)
 
 end assignment
