src/xor/tseitin_xor.lean
@@ -9,6 +9,7 @@ Carnegie Mellon University
 import cnf.literal
 import cnf.clause
 import cnf.cnf
+import cnf.encoding
 import cnf.gensym
 import xor.xor
 import xor.direct_xor
@@ -24,6 +25,7 @@ open literal
 open clause
 open cnf
 open nxor
+open encoding
 
 open list
 open assignment
@@ -61,7 +63,7 @@ begin
   exact nat.succ_le_iff.mp hk,
 end
 
--- Note: x and g can be made implicit args, but explicit feels better
+-- Note: x and g can be made implicit args
 def linear_xor {k : nat} (hk : k ≥ 3) : Π (x : nxor V), Π (g : gensym V),
   (disjoint g.stock x.vars) → cnf V
 | x g hdis := if h : length x ≤ k then direct_xor x else
@@ -75,26 +77,73 @@ using_well_founded {
   dec_tac := tactic.assumption
 }
 
-/-
-def linear_xor2 {k : nat} (hk : k ≥ 3) (x : nxor V) (g : gensym V)
-  (hg : disjoint g.stock x.vars) : nxor V → cnf V
-| x₁ := if h : length x₁ ≤ k then direct_xor x₁ else
-                have length ((Pos g.fresh.1) :: (x₁.drop k)) < length x₁,
-                  from (drop_len_lt _ hk (not_le.mp h)),
-                (direct_xor (x₁.take k ++ [(Neg g.fresh.1)])) ++
-                (linear_xor2 ((Pos g.fresh.1) :: (x₁.drop k)))
-using_well_founded {
-  rel_tac := λ a b, `[exact ⟨_, measure_wf (λ σ, list.length σ)⟩],
-  dec_tac := tactic.assumption
-}
--/
-
 lemma linear_base_case {k : nat} (hk : k ≥ 3) {x : nxor V} {g : gensym V}
   (hdis : disjoint g.stock x.vars) : 
   length x ≤ k → linear_xor hk x g hdis = direct_xor x :=
 assume h, by { rw linear_xor, simp only [h, if_true] }
 
-lemma eqsat_forward {k : nat} (hk : k ≥ 3) {x : nxor V} {g : gensym V}
+theorem mem_linear_xor_vars_of_mem_vars {k : nat} (hk : k ≥ 3) {x : nxor V} {g : gensym V}
+  (hdis : disjoint g.stock x.vars) {v : V} :
+  v ∈ x.vars → v ∈ (linear_xor hk x g hdis).vars :=
+begin
+  induction x using strong_induction_on_lists with x ih generalizing g,
+  by_cases hx : length x ≤ k,
+  { rw linear_base_case hk hdis hx, rw vars_direct_xor, exact id },
+  { intro h,
+    rw linear_xor,
+    simp [hx],
+    rw [← take_append_drop (k - 1) x, vars, clause.vars_append] at h,
+    rw cnf.vars_append,
+    rcases finset.mem_union.mp h with (h | h),
+    { apply finset.mem_union_left,
+      rw [vars_direct_xor, vars, clause.vars_append],
+      exact finset.mem_union_left _ h },
+    { rw not_le at hx,
+      have h₁ := drop_len_lt (Pos g.fresh.1) hk hx,
+      have h₂ := disjoint_fresh_of_disjoint hk hdis,
+      have := ih _ h₁ h₂ (clause.mem_vars_cons_of_mem_vars _ h),
+      exact finset.mem_union_right _ this } }
+end
+
+theorem not_mem_linear_xor_vars_of_not_mem_vars_of_not_mem_stock {k : nat} (hk : k ≥ 3) {x : nxor V} {g : gensym V}
+  (hdis : disjoint g.stock x.vars) {v : V} :
+  v ∉ x.vars → v ∉ g.stock → v ∉ (linear_xor hk x g hdis).vars :=
+begin
+  induction x using strong_induction_on_lists with x ih generalizing g,
+  by_cases hx : length x ≤ k,
+  { rw [linear_base_case hk hdis hx, vars_direct_xor x], tautology },
+  { intros hvars hg,
+    rw linear_xor,
+    simp [hx],
+    rw cnf.vars_append,
+    apply finset.not_mem_union.mpr,
+    rw vars at hvars,
+    split,
+    { rw [vars_direct_xor, vars, clause.vars_append],
+      apply finset.not_mem_union.mpr,
+      split,
+      { intro hcon,
+        have := (clause.vars_subset_of_subset (take_subset (k - 1) x)),
+        exact absurd (this hcon) hvars },
+      { simp [var],
+        intro hcon,
+        rw hcon at hg,
+        exact absurd (gensym.fresh_mem_stock g) hg } },
+    { have h₁ := drop_len_lt (Pos g.fresh.1) hk (not_le.mp hx),
+      have h₂ := disjoint_fresh_of_disjoint hk hdis,
+      have h₃ : v ∉ vars (Pos g.fresh.1 :: drop (k - 1) x),
+      { simp [vars, clause.vars, var],
+        rintros (rfl | h),
+        { exact hg (gensym.fresh_mem_stock g) },
+        { exact hvars (vars_subset_of_subset (drop_subset (k - 1) x) h) } },
+      have h₄ : v ∉ g.fresh.2.stock,
+      { intro hcon,
+        exact hg ((gensym.fresh_stock_subset g) hcon) },
+      exact ih _ h₁ h₂ h₃ h₄ } }
+end
+
+-- A slightly stronger statement
+lemma linear_forward {k : nat} (hk : k ≥ 3) {x : nxor V} {g : gensym V}
   (hdis : disjoint g.stock x.vars) {α : assignment V} :
   cnf.eval α (linear_xor hk x g hdis) = tt → cnf.eval α (direct_xor x) = tt :=
 begin
@@ -126,363 +175,207 @@ begin
       exact this.symm } }
 end
 
-lemma eqsat_backward {k : nat} (hk : k ≥ 3) {x : nxor V} {g : gensym V}
-  (hdis : disjoint g.stock x.vars) {α : assignment V} :
-  cnf.eval α (direct_xor x) = tt → (∃ (α₂ : assignment V), 
-  cnf.eval α₂ (linear_xor hk x g hdis) = tt ∧ eqod α α₂ x.vars) :=
-begin
-  induction x using strong_induction_on_lists with x ih generalizing g α,
-  by_cases hx : length x ≤ k,
-  { intro h, use α, rw linear_base_case hk hdis hx,
-    exact ⟨h, eqod.refl _ _⟩ },
-  { intro h,
-
-    rw [eval_direct_xor_eq_eval_nxor, eval_eq_bodd_count_tt] at h,
-    have := take_append_drop (k - 1) x,
-    rw [← this, count_tt_append, nat.bodd_add] at h,
-
-    -- Proof that fresh not in x.vars
-    have := set.disjoint_left.mp hdis (gensym.fresh_mem_stock g),
-
-
-    have h₁ := drop_len_lt (Pos g.fresh.1) hk (not_le.mp hx),
-    have h₂ := disjoint_fresh_of_disjoint hk hdis,
-    have ihred := ih _ h₁ h₂,
-
-
-
-    cases hc : nat.bodd (clause.count_tt α (take (k - 1) x)),
-    {
-      rw [hc, ff_bxor] at h,
-      have : clause.count_tt (assignment.ite (nxor.vars x) α all_ff) ((Pos g.fresh.1) :: (drop (k - 1) x)) = clause.count_tt α (drop (k - 1) x),
-      {
-        rw count_tt_cons,
-
-      }
-    },
-    {
-
-    }
-
-
-
-  }
-end
-
-theorem linear_xor_eqsat {k : nat} (hk : k ≥ 3) {x : nxor V} {g : gensym V}
+theorem linear_sequiv {k : nat} (hk : k ≥ 3) {x : nxor V} {g : gensym V}
   (hdis : disjoint g.stock x.vars) :
-  assignment.eqsat (λ α, cnf.eval α (linear_xor hk x g hdis)) 
-                   (λ α, cnf.eval α (direct_xor x)) :=
+  sequiv (linear_xor hk x g hdis) (direct_xor x) x.vars :=
 begin
-  split,
-  { rintros ⟨α, hl⟩,
-    use α, simp at *,
-    exact eqsat_forward hk hdis hl },
-  { induction x using strong_induction_on_lists with x ih generalizing g,
-    rintros ⟨α, hd⟩,
-    simp at *,
-    by_cases hx : length x ≤ k,
-    { use α,
+  induction x using strong_induction_on_lists with x ih generalizing g,
+  by_cases hx : length x ≤ k,
+  { rw linear_base_case hk hdis hx },
+  { intro τ,
+    split,
+    -- forward direction: linear -> direct
+    { rintros ⟨σ, hl, hs⟩,
+      use [σ, linear_forward hk hdis hl, hs] },
+    -- reverse direction: direct -> linear
+    { rintros ⟨σ, he, hs⟩,
+
+      rw [eval_direct_xor_eq_eval_nxor, eval_eq_bodd_count_tt] at he,
+      have htakedrop := take_append_drop (k - 1) x,
+      have hnotmem := set.disjoint_left.mp hdis (g.fresh_mem_stock),
+      rw [← htakedrop, count_tt_append, nat.bodd_add] at he, 
+
+      have h₁ := drop_len_lt (Pos g.fresh.1) hk (not_le.mp hx),
+      have h₂ := disjoint_fresh_of_disjoint hk hdis, 
+
       rw linear_xor,
-      simp only [hx, hd, if_true] },
-    { rw linear_xor,
-      simp [hx],
-      rw not_le at hx,
-      have h₁ := drop_len_lt (Pos g.fresh.1) hk hx,
-      have h₂ := disjoint_fresh_of_disjoint hk hdis,
+      simp [hx, cnf.eval_append],
 
-      
+      cases hc : nat.bodd (clause.count_tt σ (take (k - 1) x)),
+      { simp [hc] at he,
+        rcases exists_eqod_and_eq_of_not_mem σ ff hnotmem with ⟨γ, heqod, hg⟩,
+        have : nat.bodd (clause.count_tt γ (Pos g.fresh.1 :: drop (k - 1) x)) = tt,
+        { simp only [count_tt_cons, literal.eval, hg, cond],
+          rw ← count_tt_eq_of_eqod (eqod_subset (vars_subset_of_subset (drop_subset (k - 1) x)) heqod),
+          exact he },
+        rw [← eval_eq_bodd_count_tt, ← eval_direct_xor_eq_eval_nxor] at this,
 
-      have ihred := ih _ h₁ h₂ α,
+        -- Apply the induction hypothesis
+        rcases (ih _ h₁ h₂ γ).mpr ⟨γ, this, eqod.refl _ _⟩ with ⟨γ₂, he₂, hg₂⟩,
+        have hg₂copy := hg₂,
+        rw [vars, clause.vars, var] at hg₂copy,
+        have := eqod_subset (finset.subset_union_right {g.fresh.1} (clause.vars (x.drop (k - 1)))) hg₂copy,
 
-      
-    }
-
-  }
+        have bigeqod : eqod (assignment.ite (cnf.vars (linear_xor hk (Pos g.fresh.1 :: (x.drop (k - 1))) g.fresh.2 h₂)) γ₂ γ) γ (clause.vars x),
+        {
+          intros v hv,
+          by_cases hmem : v ∈ vars (x.drop (k - 1)),
+          { rw vars at hmem,
+            have h₃ := clause.mem_vars_cons_of_mem_vars (Pos g.fresh.1) hmem,
+            have := mem_linear_xor_vars_of_mem_vars hk h₂ h₃,
+            rw ite_pos _ _ this,
+            rw hg₂ v h₃ },
+          {
+            have hdis₂ := set.disjoint_right.mp hdis hv,
+            have hne : v ≠ g.fresh.1,
+            { intro hcon,
+              rw hcon at hdis₂,
+              exact hdis₂ (gensym.fresh_mem_stock g) },
+            have : v ∉ vars (Pos g.fresh.1 :: drop (k - 1) x),
+            { simp [vars, clause.vars, var],
+              rintros (hcon | hcon),
+              { exact hne hcon },
+              { rw vars at hmem, exact hmem hcon } },
+            have hdis₃ := gensym.fresh_stock_subset g,
+            have hstock : v ∉ g.fresh.2.stock,
+            { intro hcon,
+              exact hdis₂ (hdis₃ hcon) },
+            have := not_mem_linear_xor_vars_of_not_mem_vars_of_not_mem_stock hk h₂ this hstock,
+            rw ite_neg _ _ this } },
+        
+        use assignment.ite (cnf.vars (linear_xor hk (Pos g.fresh.1 :: (x.drop (k - 1))) g.fresh.2 h₂)) γ₂ γ,
+        
+        split,
+        { split,
+          { simp [eval_direct_xor_eq_eval_nxor, eval_eq_bodd_count_tt, 
+              count_tt_append, nat.bodd_add, literal.eval, hg],
+            have : g.fresh.1 ∈ vars (Pos g.fresh.1 :: (x.drop (k - 1))),
+            { exact mem_vars_cons_self _ _ },
+            have := mem_linear_xor_vars_of_mem_vars hk h₂ this,
+            rw ite_pos _ _ this,
+            have := clause.mem_vars_cons_self (Pos g.fresh.1) (x.drop (k - 1)),
+            rw var at this,
+            rw ← (hg₂ g.fresh.1 this),
+            simp [hg],
+            have := eqod_subset (vars_subset_of_subset (take_subset (k - 1) x)) bigeqod,
+            rw count_tt_eq_of_eqod this,
+            rw ← count_tt_eq_of_eqod (eqod_subset (vars_subset_of_subset (take_subset (k - 1) x)) heqod),
+            exact hc },
+          { rw eval_eq_cnf_of_eqod (ite_eqod _ _ _),
+            exact he₂ } },
+        { exact eqod.trans (eqod.trans hs heqod) bigeqod.symm } },
+      { sorry, } } }
 end
-/-
-lemma restriction_injective {f : nat → V} (hf : injective f) :
-  injective (λ n, f (n + 1)) :=
+
+-- Note: The proofs here are symmetric with the linear encoding ones
+-- If an improvement is made to the above proofs, simplify here
+
+lemma drop_len_lt' {k : nat} {x : nxor V} (l : literal V) :
+  k ≥ 3 → length x > k → length (x.drop (k - 1) ++ [l]) < length x :=
 begin
-  intros n₁ n₂ h,
-  exact add_right_cancel ((injective.eq_iff hf).mp h)
+  have : (drop (k - 1) x ++ [l]).length = (l :: drop (k - 1) x).length,
+  { simp only [length, length_append] },
+  rw this,
+  exact drop_len_lt l
 end
 
-lemma restriction_image_subset (f : nat → V) :
-  set.range (λ n, f (n + 1)) ⊆ set.range f :=
-begin
-  intros v hv,
-  rcases set.mem_range.mp hv with ⟨y, hy⟩,
-  apply set.mem_range.mpr,
-  use [y + 1, hy]
-end
-
-lemma restriction_first {f : nat → V} (hinj : injective f) :
-  f 0 ∉ set.range (λ n, f (n + 1)) :=
+lemma disjoint_fresh_of_disjoint' {x : nxor V} {g : gensym V} {k : nat} (hk : k ≥ 3) :
+  disjoint g.stock x.vars → 
+  disjoint g.fresh.2.stock (nxor.vars (x.drop (k - 1) ++ [Pos g.fresh.1])) :=
 begin
   intro h,
-  rcases set.mem_range.mp h with ⟨y, hy⟩,
-  have := (injective.eq_iff hinj).mp hy,
-  contradiction
-end
-
-lemma restriction_disjoint {f : nat → V} {l : list (literal V)}
-  (h : (∀ v ∈ set.range f, v ∉ (clause.vars l))) :
-  ∀ v ∈ set.range (λ n, f (n + 1)), v ∉ (clause.vars l) :=
-begin
+  apply set.disjoint_right.mpr,
   intros v hv,
-  exact h v ((restriction_image_subset f) hv),
-end
-
-lemma res_disjoint {f : nat → V} {l : list (literal V)}
-  (hinj : injective f)
-  (h : (∀ v ∈ set.range f, v ∉ (clause.vars l))) :
-  ∀ v ∈ set.range (λ n, f (n + 1)), v ∉ (clause.vars (l.drop 3 ++ [Pos (f 0)])) :=
-begin
-  intros v hv,
-  have := (restriction_disjoint h) v hv,
-  have hleft : v ∉ clause.vars (drop 3 l), exact mt 
-    (λ h, vars_subset_of_subset (drop_subset 3 l) h)
-    ((restriction_disjoint h) v hv),
-  have hright : v ∉ clause.vars [Pos (f 0)],
+  simp [vars, clause.vars, clause.vars_append] at hv,
+  rcases hv with rfl | hv,
+  { rw var,
+    exact gensym.fresh_not_mem_fresh_stock g },
   { intro hcon,
-    simp [var] at hcon,
-    simp at hv, -- what is being simplified here?
-    rcases hv with ⟨y, rfl⟩,
-    have := (injective.eq_iff hinj).mp hcon,
-    contradiction },
-  exact not_mem_vars_append_of_not_mem_of_not_mem hleft hright
+    have := clause.vars_subset_of_subset (drop_subset (k - 1) x),
+    rw set.disjoint_right at h,
+    exact absurd ((gensym.fresh_stock_subset g) hcon) (h (this hv)) }
 end
 
--- Implementation using variable stock
-def txor3 : Π (l : list (literal V)), Π (f : nat → V),
-  (injective f) → (∀ v ∈ set.range f, v ∉ (clause.vars l)) → cnf V
-| [] _ _ _ := [[]]
-| l f hinj him := if h : length l ≤ 3 then xor_cnf l else
-                  have length (l.drop 3 ++ [Pos (f 0)]) < length l,
-                    from (dropn_len _ three_gt_one (not_le.mp h)),
-                  (xor_cnf (l.take 3 ++ [Neg (f 0)])) ++
-                  (txor3 (l.drop 3 ++ [Pos (f 0)]) (λ n, f (n + 1)) 
-                    (restriction_injective hinj) (res_disjoint hinj him))
+-- Note: x and g can be made implicit args
+def pooled_xor {k : nat} (hk : k ≥ 3) : Π (x : nxor V), Π (g : gensym V),
+  (disjoint g.stock x.vars) → cnf V
+| x g hdis := if h : length x ≤ k then direct_xor x else
+                have length (x.drop (k - 1) ++ [Pos g.fresh.1]) < length x,
+                  from (drop_len_lt' _ hk (not_le.mp h)),
+                (direct_xor (x.take (k - 1) ++ [(Neg g.fresh.1)])) ++
+                (pooled_xor (x.drop (k - 1) ++ [Pos g.fresh.1]) (g.fresh.2)
+                (disjoint_fresh_of_disjoint' hk hdis))
 using_well_founded {
   rel_tac := λ a b, `[exact ⟨_, measure_wf (λ σ, list.length σ.1)⟩],
   dec_tac := tactic.assumption
 }
 
-theorem txor3_eq_xor_cnf_of_len_le_three {l : list (literal V)}
-  {f : nat → V} (hinj : injective f) (him : ∀ v ∈ set.range f, v ∉ (clause.vars l)) :
-  length l ≤ 3 → (txor3 l f hinj him) = xor_cnf l :=
-begin
-  intro h,
-  cases l with l ls,
-  { simp [txor3] },
-  { unfold txor3, simp [h] }
-end
+lemma pooled_base_case {k : nat} (hk : k ≥ 3) {x : nxor V} {g : gensym V}
+  (hdis : disjoint g.stock x.vars) : 
+  length x ≤ k → pooled_xor hk x g hdis = direct_xor x :=
+assume h, by { rw pooled_xor, simp only [h, if_true] }
 
--- Switch to set version of vars across the table
--- doesn't actually work, but can say that any new variables introduced don't conflict with earlier ones
-/-
-theorem txor3_vars_disjoint (a b c : literal V) (l : list (literal V))
-  {f : nat → V} (hinj : injective f)
-  (him : ∀ v ∈ set.range f, v ∉ (clause.vars l))
-  (him₂ : ∀ v ∈ set.range f, v ∉ (clause.vars [a, b, c])) 
-  (hdis : disjoint (clause.vars [a, b, c]) (clause.vars l)) :
-  disjoint (clause.vars [a, b, c]) (cnf.vars (txor3 l f hinj him)) :=
+theorem mem_pooled_xor_vars_of_mem_vars {k : nat} (hk : k ≥ 3) {x : nxor V} {g : gensym V}
+  (hdis : disjoint g.stock x.vars) {v : V} :
+  v ∈ x.vars → v ∈ (pooled_xor hk x g hdis).vars :=
 begin
-end
--/
-
-theorem stronger (l : list (literal V)) (α : assignment V)
-  {f : nat → V} (hinj : injective f)
-  (him : ∀ v ∈ set.range f, v ∉ (clause.vars l)) :
-  cnf.eval α (xor_cnf l) = tt →
-  ∃ (α₂ : assignment V), cnf.eval α₂ (txor3 l f hinj him) = tt ∧ 
-  (α ≡[clause.vars l]≡ α₂) :=
-begin
-  induction l using strong_induction_on_lists with l ih generalizing α f,
-  by_cases hlen : length l ≤ 3,
-  { rw txor3_eq_xor_cnf_of_len_le_three hinj him hlen, 
-    intro h,
-    use α,
-    exact and.intro h (eqod.refl α _) },
+  induction x using strong_induction_on_lists with x ih generalizing g,
+  by_cases hx : length x ≤ k,
+  { rw pooled_base_case hk hdis hx, rw vars_direct_xor, exact id },
   { intro h,
-    rcases exists_three (not_le.mp hlen) with ⟨a, b, c, L, rfl⟩,
-
-    unfold txor3,
-    simp [hlen, cnf.eval_append],
-
-    have c_to_app : a :: b :: c :: L = [a, b, c] ++ L, simp,
-    have ha_in : a ∈ [a, b, c], simp,
-    have hb_in : b ∈ [a, b, c], simp,
-    have hc_in : c ∈ [a, b, c], simp,
-    have hav_in : a.var ∈ clause.vars [a, b, c],
-      from mem_vars_of_mem_clause ha_in,
-    have hbv_in : b.var ∈ clause.vars [a, b, c],
-      from mem_vars_of_mem_clause hb_in,
-    have hcv_in : c.var ∈ clause.vars [a, b, c],
-      from mem_vars_of_mem_clause hc_in,
-
-    rw [c_to_app, eval_xor_cnf_eq_eval_nxor, nxor.eval_append] at h,
-    
-    --have ihred := ih (L ++ [Pos (f 0)]) (dropn_len _ three_gt_one (not_le.mp hlen)) 
-    --  (restriction_injective hinj) (res_disjoint hinj him),
-
-    cases h3eval : nxor.eval α [a, b, c],
-    { simp [h3eval] at h,
-      have heval : literal.eval (set_var α (f 0) ff) (Pos (f 0)) = ff,
-      { simp [literal.eval, set_var] },
-
-      have hf0_not_mem : (f 0) ∉ clause.vars L,
-      { simp at him,
-        rw c_to_app at him,
-        intro h,
-        exact (him 0) ((vars_append_subset_right _ _) h) },
-
-      have hf0_not_mem2 : (f 0) ∉ clause.vars [a, b, c],
-      { simp at him,
-        rw c_to_app at him,
-        intro h,
-        exact (him 0) ((vars_append_subset_left _ _) h) },
-
-      have hf0_mem : (f 0) ∈ clause.vars (L ++ [Pos (f 0)]),
-      { have : f 0 ∈ clause.vars [Pos (f 0)],
-          by simp [clause.vars, literal.var],
-        exact (vars_append_subset_right L _) this },
-
-      have : cnf.eval (set_var α (f 0) ff) (xor_cnf (L ++ [Pos (f 0)])) = tt,
-      { rw eval_xor_cnf_eq_eval_nxor,
-        rw nxor.eval_append,
-        simp [literal.eval, heval],
-        have : α ≡[clause.vars L]≡ (set_var α (f 0) ff),
-          from eqod_set_var_of_not_mem α (f 0) ff (clause.vars L) hf0_not_mem,
-        rw ← equiv_on_domain_for_xor this,
-        exact h },
-      
-      have ihred := ih (L ++ [Pos (f 0)]) (dropn_len _ three_gt_one (not_le.mp hlen))
-        (set_var α (f 0) ff)
-        (restriction_injective hinj) (res_disjoint hinj him) this,
-      
-      rcases ihred with ⟨α₂, ha₂, heqod⟩,
-      use (assignment.ite α α₂ (clause.vars [a, b, c])),
-      split,
-      {
-        split,
-        { have : [a, b, c, Neg (f 0)] = [a, b, c] ++ [Neg (f 0)], simp,
-          rw [this, eval_xor_cnf_eq_eval_nxor, nxor.eval_append],
-          rw nxor.eval_singleton,
-          simp [nxor.eval_cons, literal.eval],
-          rw ite_pos_of_lit _ _ hav_in, -- This is overly manual...
-          rw ite_pos_of_lit _ _ hbv_in,
-          rw ite_pos_of_lit _ _ hcv_in,
-          rw ite_neg _ _ hf0_not_mem2,
-          rw ← heqod (f 0) hf0_mem,
-          simp [set_var],
-          rw ← bxor_tt_right (literal.eval α c),
-          simp only [← bool.bxor_assoc],
-          rw bxor_tt_right,
-          simp [nxor.eval_cons] at h3eval,
-          simp [h3eval] },
-        {
-          -- Theorems on variables, subsets, etc.
-          sorry,
-        } },
-      { intros v hv,
-        unfold assignment.ite,
-        rw c_to_app at hv,
-        rcases exists_mem_clause_of_mem_vars hv with ⟨lit, hlit, rfl⟩,
-        rcases mem_append.mp hlit with hl | hl,
-        { simp [mem_vars_of_mem_clause hl] },
-        { have hsetvar := heqod lit.var (mem_vars_of_mem_clause (mem_append_left [Pos (f 0)] hl)),
-          unfold set_var at hsetvar,
-          have := mem_vars_of_mem_clause hl,
-          have := ne_of_mem_of_not_mem this hf0_not_mem,
-          simp [this] at hsetvar,
-          simp [hsetvar] } } },
-    { -- symmetric to other case
-      sorry,
-    } }
+    rw pooled_xor,
+    simp [hx],
+    rw [← take_append_drop (k - 1) x, vars, clause.vars_append] at h,
+    rw cnf.vars_append,
+    rcases finset.mem_union.mp h with (h | h),
+    { apply finset.mem_union_left,
+      rw [vars_direct_xor, vars, clause.vars_append],
+      exact finset.mem_union_left _ h },
+    { rw not_le at hx,
+      have h₁ := drop_len_lt' (Pos g.fresh.1) hk hx,
+      have h₂ := disjoint_fresh_of_disjoint' hk hdis,
+      have h₃ : v ∈ vars (drop (k - 1) x ++ [Pos g.fresh.1]),
+      { rw [vars, clause.vars_append],
+        exact finset.mem_union_left _ h },
+      have := ih _ h₁ h₂ h₃,
+      exact finset.mem_union_right _ this } }
 end
 
-theorem backward (l : list (literal V)) {f : nat → V} (hinj : injective f)
-  (him : ∀ v ∈ set.range f, v ∉ (clause.vars l)) :
-  (∃ (α : assignment V), cnf.eval α (xor_cnf l) = tt) → 
-  ∃ (α₂ : assignment V), cnf.eval α₂ (txor3 l f hinj him) = tt :=
+theorem not_mem_pooled_xor_vars_of_not_mem_vars_of_not_mem_stock {k : nat} (hk : k ≥ 3) {x : nxor V} {g : gensym V}
+  (hdis : disjoint g.stock x.vars) {v : V} :
+  v ∉ x.vars → v ∉ g.stock → v ∉ (pooled_xor hk x g hdis).vars :=
 begin
-  rintros ⟨α, ha⟩,
-  rcases stronger l α hinj him ha with ⟨α₂, ha₂, _⟩,
-  use [α₂, ha₂]
-end
-
-theorem stronger_forward (l : list (literal V)) (α : assignment V)
-  {f : nat → V} (hinj : injective f)
-  (him : ∀ v ∈ set.range f, v ∉ (clause.vars l)) :
-  cnf.eval α (txor3 l f hinj him) = tt →
-  ∃ (α₂ : assignment V), cnf.eval α₂ (xor_cnf l) = tt ∧
-  (α ≡[clause.vars l]≡ α₂) :=
-begin
-  induction l using strong_induction_on_lists with l ih generalizing f,
-  by_cases hlen : length l ≤ 3,
-  { rw txor3_eq_xor_cnf_of_len_le_three hinj him hlen,
-    intro h, use [α, h] },
-  { rcases exists_three (not_le.mp hlen) with ⟨a, b, c, L, rfl⟩,
-    unfold txor3,
-    simp [hlen, cnf.eval_append],
-    intros h₁ h₂,
-
-    have ihred := ih (L ++ [Pos (f 0)]) (dropn_len _ three_gt_one (not_le.mp hlen))
-      (restriction_injective hinj) (res_disjoint hinj him) h₂,
-    
-    rcases ihred with ⟨α₂, ha₂, heqod⟩,
-    use α,
+  induction x using strong_induction_on_lists with x ih generalizing g,
+  by_cases hx : length x ≤ k,
+  { rw [pooled_base_case hk hdis hx, vars_direct_xor x], tautology },
+  { intros hvars hg,
+    rw pooled_xor,
+    simp [hx],
+    rw cnf.vars_append,
+    apply finset.not_mem_union.mpr,
+    rw vars at hvars,
     split,
-    { have c_to_app : a :: b :: c :: L = [a, b, c] ++ L, simp,
-      rw c_to_app,
-      have : f 0 ∈ clause.vars ([Pos (f 0)]),
-        by simp [literal.var],
-      have hf0_mem := (vars_append_subset_right L [Pos (f 0)]) this,
-      have hf0_eval := heqod (f 0) hf0_mem,
-
-      have heqod₂ := eqod_subset_of_eqod (vars_append_subset_left L ([Pos (f 0)])) heqod,
-
-      rw eval_xor_cnf_eq_eval_nxor,
-      rw eval_xor_cnf_eq_eval_nxor at h₁,
-      rw eval_xor_cnf_eq_eval_nxor at ha₂,
-      rw nxor.eval_append,
-      rw nxor.eval_append at ha₂,
-      cases heval : α₂ (f 0),
-      { simp [literal.eval, heval] at ha₂,
-        simp only [nxor.eval_cons, literal.eval, heval, hf0_eval] at h₁,
-        rw nxor.eval_nil at h₁,
-        rw bool.bxor_ff_right at h₁,
-        simp only [← bool.bxor_assoc] at h₁, -- clean up manual
-        rw bool.bnot_false at h₁,
-        rw bxor_tt_right at h₁,
-        simp at h₁,
-        rw equiv_on_domain_for_xor heqod₂,
-        simp [ha₂, nxor.eval_cons, h₁] },
-      {
-        simp [literal.eval, heval] at ha₂,
-        simp only [nxor.eval_cons, literal.eval, heval, hf0_eval] at h₁,
-        rw nxor.eval_nil at h₁,
-        rw bool.bxor_ff_right at h₁,
-        simp only [← bool.bxor_assoc] at h₁, -- clean up manual
-        rw bool.bnot_true at h₁,
-        rw bool.bxor_ff_right at h₁,
-        simp at h₁,
-        rw equiv_on_domain_for_xor heqod₂,
-        simp [ha₂, nxor.eval_cons, h₁] } },
-    { exact eqod.refl α _ } }
+    { rw [vars_direct_xor, vars, clause.vars_append],
+      apply finset.not_mem_union.mpr,
+      split,
+      { intro hcon,
+        have := (clause.vars_subset_of_subset (take_subset (k - 1) x)),
+        exact absurd (this hcon) hvars },
+      { simp [var],
+        intro hcon,
+        rw hcon at hg,
+        exact absurd (gensym.fresh_mem_stock g) hg } },
+    { have h₁ := drop_len_lt' (Pos g.fresh.1) hk (not_le.mp hx),
+      have h₂ := disjoint_fresh_of_disjoint' hk hdis,
+      have h₃ : v ∉ vars (drop (k - 1) x ++ [Pos g.fresh.1]),
+      { simp [vars, clause.vars, var, clause.vars_append],
+        rintros (h | rfl),
+        { exact hvars (vars_subset_of_subset (drop_subset (k - 1) x) h) },
+        { exact hg (gensym.fresh_mem_stock g) } },
+      have h₄ : v ∉ g.fresh.2.stock,
+      { intro hcon,
+        exact hg ((gensym.fresh_stock_subset g) hcon) },
+      exact ih _ h₁ h₂ h₃ h₄ } }
 end
-
-theorem forward (l : list (literal V)) {f : nat → V} (hinj : injective f)
-  (him : ∀ v ∈ set.range f, v ∉ (clause.vars l)) :
- (∃ (α : assignment V), cnf.eval α (txor3 l f hinj him) = tt) → 
-  ∃ (α₂ : assignment V), cnf.eval α₂ (xor_cnf l) = tt :=
-begin
-  rintros ⟨α, ha⟩,
-  rcases stronger_forward l α hinj him ha with ⟨α₂, ha₂, _⟩,
-  use [α₂, ha₂]
-end
--/
 
 end tseitin_xor
