src/cnf/encoding.lean
@@ -1,0 +1,61 @@
+/-
+This file sets out definitions of what it means for a CNF formula to encode
+a Boolean function. Encodings of non-Boolean functions may require different
+definitions.
+
+Authors: Cayden Codel, Marijn Heule, Jeremy Avigad
+Carnegie Mellon University
+-/
+
+import cnf.literal
+import cnf.assignment
+import cnf.clause
+import cnf.cnf
+import basic
+
+universe u
+
+variables {V : Type*} [decidable_eq V] [inhabited V]
+
+namespace encoding
+
+open assignment
+
+/- A CNF formula encodes a Boolean function -/
+def encodes (f : list bool → bool) (F : cnf V) (s : list V) :=
+  ∀ τ, (f (s.map τ) = tt ↔ ∃ σ, F.eval σ = tt ∧ (τ ≡s.to_finset≡ σ))
+
+/- Definition of S-equivalence -/
+def sequiv (F₁ F₂ : cnf V) (s : finset V) := ∀ τ, 
+  ((∃ σ₁, F₁.eval σ₁ = tt ∧ (τ ≡s≡ σ₁)) ↔ (∃ σ₂, F₂.eval σ₂ = tt ∧ (τ ≡s≡ σ₂)))
+
+@[refl] theorem sequiv.refl (F : cnf V) (s : finset V) : sequiv F F s :=
+assume _, iff.rfl
+
+@[symm] theorem sequiv.symm {F₁ F₂ : cnf V} {s : finset V} :
+  sequiv F₁ F₂ s → sequiv F₂ F₁ s :=
+assume h τ, (h τ).symm
+
+@[trans] theorem sequiv.trans {F₁ F₂ F₃ : cnf V} {s : finset V} :
+  sequiv F₁ F₂ s → sequiv F₂ F₃ s → sequiv F₁ F₃ s :=
+begin
+  intros h₁ h₂ τ,
+  split,
+  { intro h,
+    exact (h₂ τ).mp ((h₁ τ).mp h) },
+  { intro h,
+    exact (h₁ τ).mpr ((h₂ τ).mpr h) }
+end
+
+theorem encodes_of_encodes_of_sequiv {f : list bool → bool} {F₁ F₂ : cnf V} (s : list V) :
+  encodes f F₁ s → sequiv F₁ F₂ s.to_finset → encodes f F₂ s :=
+begin
+  intros h₁ h₂ τ,
+  split,
+  { intro hf,
+    exact (h₂ τ).mp ((h₁ τ).mp hf) },
+  { intro h,
+    exact (h₁ τ).mpr ((h₂ τ).mpr h) }
+end
+
+end encoding
